contracts discovery and contract message generation WIP

ContractExamples.Tests/Tests.fs
@@ -1,0 +1,138 @@
+﻿module Tests
+
+open NUnit.Framework
+open ContractExamples
+open ContractExamples.FStarCompatibility
+open Consensus.Types
+open Zen.Types.Extracted
+open Consensus.Serialization
+open System.IO
+
+open ContractExamples.FStarExecution
+
+let readContract fileName =
+    System.IO.File.ReadAllText(Path.Combine (resolvePath "../../FStar", Path.ChangeExtension(fileName, ".fst")))
+
+let getContractFunction contract =
+    let extracted = readContract contract |> extract
+    Assert.IsTrue ((Option.isSome extracted), "Should extract")
+
+    let compiled = extracted |> Option.get |> compile 
+    Assert.NotNull (compiled, "Should compile") // https://stackoverflow.com/questions/10435052/f-passing-none-to-function-getting-null-as-parameter-value
+    Assert.That ((Option.isSome compiled), "Should compile")
+
+    let func = compiled |> Option.get |> deserialize
+    Assert.That ((Option.isSome func), "Should deserialize")
+
+    Option.get func
+
+let createHash b : Hash = Array.map (fun x -> b) [|0..31|]
+       
+//TODO: huh?
+context.Serializers.RegisterOverride<data<unit>>(new DataSerializer(context))
+
+
+open ContractExamples.QuotedContracts
+open ContractUtilities
+open ContractExamples.Execution
+open ResultWorkflow
+
+[<Test>]
+let ``TestCallOptionMessageComposition``() =
+    let func = getContractFunction "CallOption"
+
+    let numeraire = createHash 0uy
+    let contractHash = createHash 5uy
+    let txHash = createHash 10uy
+    let amount = 50UL
+
+    let meta = CallOption {
+        numeraire = Consensus.Tests.zhash;
+        controlAsset = [||];
+        controlAssetReturn = [||];
+        oracle = [||];
+        underlying = "GOOG";
+        price = 10m;
+        strike = 10m;
+        minimumCollateralRatio = 1m;
+        ownerPubKey = [||]
+    }
+
+    let utxos = []
+        //[({ 
+        //    Consensus.Types.txHash = txHash
+        //    index = 199ul
+        //}, {
+        //    Consensus.Types.lock = Consensus.Types.PKLock contractHash
+        //    spend =
+        //    {
+        //        asset = Consensus.Tests.zhash
+        //        amount = amount
+        //    }
+        //})]
+
+    let utxo : ContractExamples.Execution.Utxo =
+        function 
+        | { txHash = txHash; index = 55ul } when txHash = txHash -> 
+            Some {
+                lock = Consensus.Types.PKLock contractHash 
+                spend = {
+                        asset = numeraire
+                        amount = amount 
+                    } 
+            }
+        | _ -> None
+
+    let args = Map.ofList [("", "");]
+
+    let outpoint = { Consensus.Types.txHash = txHash; index = 55ul }
+
+    // TODO: pyramid of doom!
+    let checkStateCorrectness (state:Output, collateral, tokensIssued, counter) =
+        if numeraire <> state.spend.asset then
+            Error "Invalid asset"
+        else
+            if collateral <> state.spend.amount then
+                Error "Invalid collateral"
+            else
+                match state.lock with
+                | Consensus.Types.ContractLock (hash, data) ->
+                    let serializer = context.GetSerializer<data<unit>>()
+                    match serializer.UnpackSingleObject data with
+                    | Data2 (_, _, UInt64 d1, UInt64 d2) ->
+                        if tokensIssued <> d1 then
+                            Error "Invalid tokens issued"
+                        else 
+                            if counter <> d2 then
+                                Error "Invalid counter"
+                            else
+                                Ok true //
+                    | _ -> Error "unexpected data"
+                | _ -> Error "unexpected lock type"
+
+    let getStateOutput (result:ContractResult) = 
+        match result with 
+        | Ok (outpointList, outputList, _) -> 
+            if List.isEmpty outputList then
+                Error "no outputs"
+            else
+                let fstOutput = outputList.[0]
+                match fstOutput.lock with
+                | Consensus.Types.ContractLock _ ->
+                    Ok fstOutput
+                | _ -> Error "unexpected lock type"
+        | Error msg -> 
+            Error ("contract responded with error message: " + msg)
+
+    let result = result {
+        match DataGenerator.makeJson (meta, utxos, 0uy, args) with 
+        | Ok json ->
+            let funcResult = func (DataGenerator.makeMessage (json, outpoint), contractHash, utxo)
+            let! state = getStateOutput funcResult
+            return! checkStateCorrectness (state, amount, 0UL, 1UL)
+        | Error x -> return! Error ("Message generator error: " + x.ToString())
+    }
+
+    match result with 
+    | Error x -> Assert.Fail x
+    | _ -> ignore()
