ContractUtilities/ResultWorkflow.fs
@@ -1,0 +1,53 @@
+﻿module ContractUtilities.ResultWorkflow
+
+open System
+
+    /// Forked from FSharpX -- topynate
+    /// The maybe monad.
+    /// This monad is my own and uses an 'T option. Others generally make their own Maybe<'T> type from Option<'T>.
+    /// The builder approach is from Matthew Podwysocki's excellent Creating Extended Builders series http://codebetter.com/blogs/matthew.podwysocki/archive/2010/01/18/much-ado-about-monads-creating-extended-builders.aspx.
+
+
+type ResultBuilder() =
+    member this.Return(x) = Ok x
+
+    member this.ReturnFrom(m: Result<'Err, 'Value>) = m
+
+    member this.Bind(m, f) = Result.bind f m
+
+    member this.Bind((e, opt): 'Err * 'T option, f) = Result.bind f (match opt with 
+                                                                       | Some x -> Ok x 
+                                                                       | None -> Error e)
+
+    member this.Zero() = this.Return ()
+
+    member this.Combine(m, f) = Result.bind f m
+
+    member this.Delay(f: unit -> _) = f
+
+    member this.Run(f) = f()
+
+    //member this.TryWith(m, h) =
+    //    try this.ReturnFrom(m())
+    //    with e -> h e
+
+    //member this.TryFinally(m, compensation) =
+    //    try this.ReturnFrom(m())
+    //    finally compensation()
+
+    //member this.Using(res:#IDisposable, body) =
+    //    let body' = fun () -> body res
+    //    this.TryFinally(body', fun () ->
+    //        match res with
+    //        | null -> ()
+    //        | disp -> disp.Dispose())
+
+    //member this.While(guard, f) =
+    //    if not (guard()) then Some () else
+    //    do f() |> ignore
+    //    this.While(guard, f)
+
+    //member this.For(sequence:seq<_>, body) =
+        //this.Using(sequence.GetEnumerator(),
+                             //fun enum -> this.While(enum.MoveNext, this.Delay(fun () -> body enum.Current)))
+let result = ResultBuilder()
